\documentclass[letterpaper, 12pt]{article}
\usepackage{amsmath, amssymb}

\newtheorem{theorem}{Theorem}[section]
\newtheorem{lemma}[theorem]{Lemma}
\newtheorem{proposition}[theorem]{Proposition}
\newtheorem{corollary}[theorem]{Corollary}

\newenvironment{proof}[1][Proof]{\begin{trivlist}
\item[\hskip \labelsep {\bfseries #1}]}{\end{trivlist}}
\newenvironment{definition}[1][Definition]{\begin{trivlist}
\item[\hskip \labelsep {\bfseries #1}]}{\end{trivlist}}
\newenvironment{example}[1][Example]{\begin{trivlist}
\item[\hskip \labelsep {\bfseries #1}]}{\end{trivlist}}
\newenvironment{remark}[1][Remark]{\begin{trivlist}
\item[\hskip \labelsep {\bfseries #1}]}{\end{trivlist}}

\newcommand{\qed}{\quad \blacksquare}
\newcommand{\keyword}[1]{\textbf{#1}}
\newcommand{\then}{\rightarrow}
\newcommand{\bithen}{\leftrightarrow}

\title{MATH 381 Homework 5}
\author{Olivia Dumitrescu}
\date{17 February 2024}

\begin{document}
\maketitle
\begin{enumerate}
\item Suppose that $x$ and $y$ are real numbers. Prove that if $x + y$ is irrational then $x$ is 
irrational or $y$ is irrational.
\begin{align*}
    x, y& \in \mathbb{R} \\
    p:& \quad x + y \notin \mathbb{Q} \\
    q:& \quad x \notin \mathbb{Q} \vee y \notin \mathbb{Q}
\end{align*}
\begin{gather*}
    p \then q \equiv \neg q \then \neg p
\end{gather*}
\begin{align*}
    \neg p:& \quad x + y \in \mathbb{Q} \\
    \neg q:& \quad x \in \mathbb{Q} \wedge y \in \mathbb{Q}
\end{align*}
\begin{flushleft}
    Suppose $\neg q$.
\end{flushleft}
\begin{align*}
    x = \frac{a}{b} & \quad y = \frac{c}{d} &\quad a, b, c, d \in \mathbb{Z} &\quad b, d \ne 0 \\
    x + y = \frac{a}{b} + \frac{c}{d} &= \frac{ad}{bd} + \frac{bc}{bd} = \frac{ad + bc}{bd}
    = \frac{e}{f} &\quad e, f \in \mathbb{Z} &\quad f \ne 0 \\
    & & \therefore \frac{e}{f} = x + y \in \mathbb{Q} \qed
\end{align*}
\begin{flushleft}
    Therefore, $\neg q \then \neg p \equiv p \then q$.
\end{flushleft}
\pagebreak
\item Show that any integer is a multiple of 3 if and only if its square is a multiple of 3.
\begin{flushleft}
    $P(n)$: ``$n$ is a multiple of 3'' $\equiv \exists k \in \mathbb{Z} (n = 3k)$ \\
    $Q(n)$: ``$n^2$ is a multiple of 3'' $\equiv \exists m \in \mathbb{Z} (n^2 = 3m)$ 
\end{flushleft}
\begin{multline*}
    \forall n \in \mathbb{Z} (P(n) \leftrightarrow Q(n)) \\
    \equiv \forall n \in \mathbb{Z} (P(n) \then Q(n)) \wedge \forall n \in \mathbb{Z}(Q(n) \then P(n))
\end{multline*}
Suppose $P(n)$.
\begin{gather*}
    n = 3k \quad k \in \mathbb{Z} \\
    n^2 = (3k)^2 = (3^2 k^2) = 3(3k^2) = 3m \quad m = 3k^2 \in \mathbb{Z}
\end{gather*}
$\therefore Q(n)$ \\
Suppose $Q(n)$.
\begin{gather*}
    n^2 = 3m \quad m \in \mathbb{Z} \\
    \sqrt{n^2} = \sqrt{3m} = \sqrt{3}\sqrt{m} \\
\end{gather*}
Since $n^2$ is a square of an integer:
\begin{align*}
    & \sqrt{n^2} \in \mathbb{Z}_+ \\
    &\implies \sqrt{3}\sqrt{m} \in \mathbb{Z}_+ \\
    &\implies \sqrt{3}\sqrt{3}\sqrt{m/3} \in \mathbb{Z}_+ \\
    &\implies 3\sqrt{m/3} \in \mathbb{Z}_+ \\
    &\implies \sqrt{m/3} \in \mathbb{Z}_+ \because 3 \in \mathbb{Z}_+ \\
    &\therefore \sqrt{n^2} = n = 3k \quad \sqrt{m/3} = k \in \mathbb{Z}_+
\end{align*}
$\therefore P(n) \qed$
\pagebreak
\item Using the definition $|x| = \begin{cases}
    \; x \quad \text{ if } x \ge 0 \\
    -x \quad \text{ if } x < 0
\end{cases}$, 
prove that for all real numbers $x$ and $y$, $|x| \le y$ if and only if $-y \le x \le y$.
\begin{flushleft}
    $P(x, y)$: $|x| \le y$ \\
    $Q(x, y)$: $-y \le x \le y$
\end{flushleft}
\[\forall x, y \in \mathbb{R}(P(x, y) \leftrightarrow Q(x, y))\]
Suppose $P(x, y)$.
\begin{gather*}
    |x| \le y = \begin{cases}
        x \le y \quad \text{ if } x \ge 0 \\
        -x \le y \quad \text{ if } x < 0
    \end{cases} = \begin{cases}
        x \le y \quad \text{ if } x \ge 0 \\
        x \ge -y \quad \text{ if } x < 0
    \end{cases}
\end{gather*}
\begin{align*}
    &\iff (x \le y \wedge x \ge 0) \vee (x \ge -y \wedge x < 0) \\
    &\iff (0 \le x \le y) \vee (-y \le x < 0) \\
    &\iff x \in [0, y] \vee x \in [-y, 0) \\
    &\iff x \in [0, y] \cup [-y, 0) \\
    &\iff x \in [-y, y] \\
    &\iff -y \le x \le y
\end{align*}
$\therefore Q(x, y) \qed$
\pagebreak
\item Prove that if $ab > 0$ and $bc < 0$, then $ax^2 + bx + c = 0$ has two real solutions.
\[x = \frac{-b \pm \sqrt{b^2 - 4ac}}{2a}\]
The quadratic equation has two real solutions when $b^2 - 4ac > 0 \iff b^2 > 4ac$.
\begin{gather*}
    (ab > 0) \then (a > 0 \wedge b > 0) \vee (a < 0 \wedge b < 0) \\
    (bc < 0) \then (b < 0 \wedge c > 0) \vee (b > 0 \wedge c < 0)
\end{gather*}
\begin{flushleft}
    There are two possibilities, since $a$ and $c$ are dependent on the value of $b$ to fulfill 
    their inequalities. \\ If $b$ is negative, then $a$ must be negative as well, and 
    $c$ must be positive. \\ If $b$ is positive, then $a$ must be positive as well, and $c$ 
    must be negative.
\end{flushleft}
\begin{gather*}
    (b > 0) \then (a > 0 \wedge c < 0) \\
    (b < 0) \then (a < 0 \wedge c > 0)
\end{gather*}
Assume $b < 0$.
\begin{gather*}
    b^2 > 0 \\
    a < 0 \implies 4ac < 0 \\
    \therefore b^2 > 4ac
\end{gather*}
Assume $b > 0$.
\begin{gather*}
    b^2 > 0 \\
    c < 0 \implies 4ac < 0 \\
    \therefore b^2 > 4ac
\end{gather*}
\[(ab > 0 \wedge bc < 0) \then (b^2 - 4ac > 0) \qed\]
\pagebreak
\item Prove that there are no positive integer solutions to $x^2 + x + 1 = y^2$.
\begin{align*}
    \neg(\exists x \in \mathbb{Z}_+ \exists y \in \mathbb{Z}_+(x^2 + x + 1 = y^2)) \\
    \forall x \in \mathbb{Z}_+ \forall y \in \mathbb{Z}_+(x^2 + x + 1 \ne y^2)
\end{align*}
Assume $x, y \in \mathbb{Z}_+$.
\begin{align*}
    y^2 - x^2 &= x + 1 \\
    \implies (y + x)(y - x) &= x + 1
\end{align*}
There are three possible cases for $x$ and $y$
\begin{enumerate}
    \item $y = x$
    \begin{align*}
        (y + x)(y - x) &= x + 1 \\
        \implies 2y(0) &= y + 1 \\
        0 &= y + 1 \equiv F \because y > 0
    \end{align*}
    \item $y < x$
    \begin{align*}
        (y + x)(y - x) &= x + 1 \\
        (y + x)(y - x) &< 0 \because (y + x) > 0 \wedge (y - x < 0 \iff y < x) \\
        x + 1 &> 0 \because x > 0 \\
        \therefore (y + x)(y - x) = x + 1 \equiv F
    \end{align*}
    \item $y > x$
    \begin{align*}
        x^2 + x + 1 &= y^2 \\
        x^2 + x + \frac{1}{4} + 1 - \frac{1}{4} &= y^2 \\
        (x + \frac{1}{2})^2 + \frac{3}{4} &= y^2 \\
        (x + \frac{1}{2})^2 + \frac{3}{4} &\notin \mathbb{Z} \\
        \implies (x + \frac{1}{2})^2 + \frac{3}{4} &= y^2 \equiv F \qed
    \end{align*}
\begin{flushleft}
    Since in all three cases for positive integer solutions or $x$ and $y$ the proposition we 
    are trying to prove implies a contradiction, the assumption that there are positive integer 
    solutions must be false.
\end{flushleft}
\end{enumerate}
\pagebreak
\item Show that if you choose 92 different dates from a calendar, at least 14 of the chosen 
dates must occur on the same day of the week.
\begin{flushleft}
    $r$: ``If you choose 92 different dates from a calendar.'' \\
    $p$: ``At least 14 of the 92 chosen dates must occur on the same day of the week.'' \\
    $\neg p$: ``At most 13 of the 92 chosen days fall on the same day of the week.'' \\
    Suppose $\neg p$. Since there are 7 days in a week, 13 on each day would give us 91 total 
    chosen days. Any more days chosen necessarily means that there would be a fourteenth date 
    on a given day of the week. But we have to choose 92 dates. This suggests 
    $\neg p \then (r \wedge \neg r)$ is true. In other words, if $p$ was false, it would imply 
    a contradiction. Therefore, $p$ must be true, and $p$ is dependent on $r$ for the number of 
    chosen dates that was agreed upon (92). So, $r \then p$ is true. $\qed$
\end{flushleft}
\pagebreak
\item Show that there is a three-digit number less than 400 with distinct digits such that 
the sum of the digits is 17 and the product of the digits is 108. Is there a unique such number? 
Explain.
\begin{gather*}
    n = 100n_2 + 10n_1 + 1n_0 < 400 \\
    n_2 + n_1 + n_0 = 17 \\
    n_2 \cdot n_1 \cdot n_0 = 108 \\
    108 = 12 \cdot 9 = 3 \cdot 4 \cdot 3^2 = 2^2 \cdot 3^3 \\
    n_1, n_2, n_3 \ne 0 \because n_2 \cdot n_1 \cdot n_0 = 108 \ne 0
\end{gather*}
\begin{center}
    \begin{tabular}{c | c | c | c | c}
        $i$ & $j$ & $2^i$ & $3^j$ & $2^i \cdot 3^j$ \\
        0 & 0 & 1 & 1 & *1 \\
        0 & 1 & 1 & 3 & *3 \\
        0 & 2 & 1 & 9 & *9 \\
        0 & 3 & 1 & 27 & 27 \\
        1 & 0 & 2 & 1 & *2 \\
        1 & 1 & 2 & 3 & *6 \\
        1 & 2 & 2 & 9 & 18 \\
        1 & 3 & 2 & 27 & 54 \\
        2 & 0 & 4 & 1 & *4 \\
        2 & 1 & 4 & 3 & 12 \\
        2 & 2 & 4 & 9 & 36 \\
        2 & 3 & 4 & 27 & 108 \\
    \end{tabular}
\end{center}
\begin{gather*}
    n_1, n_2, n_3 \in \{1, 2, 3, 4, 6, 9\} \\
    6 + 3 + 4 = 13 < 17 \implies (n_1 = 9) \vee (n_2 = 9) \vee (n_3 = 9) \\
    17 - 9 = 8 = 6 + 2 \\
    n_1, n_2, n_3 \in \{2, 6, 9\} \\
    n_2 \ne 9 \because n \ge 900 > 400 \\
    n_2 \ne 6 \because n \ge 600 > 400 \\
    \implies n_2 = 2
    (n_2 = 2 \wedge n_1 = 6 \wedge n_0 = 9) \then (n = 269) \\
    (n = 269) \then (n < 400) \\
    \therefore (n_2 = 2 \wedge n_1 = 6 \wedge n_0 = 9) \then (n < 400)
    (n_2 = 2 \wedge n_1 = 9 \wedge n_0 = 6) \then (n = 296) \\
    (n = 296) \then (n < 400) \\
    \therefore (n_2 = 2 \wedge n_1 = 9 \wedge n_0 = 6) \then (n < 400) \qed
\end{gather*}
\begin{flushleft}
    \textbf{Yes, there is such a number}. One such number is 269. Its digits were found by finding 
    combinations of factors in the prime factorization in 108 that could possibly add to 17. 
    9 must be a digit to reach 17 as a sum, and the only other factors that add to 8 are 2 and 
    6. Since 6 and 9 as the first digit would make the number greater than 400, 2 must be the 
    first digit, and a possible number was revealed to be 269 which is indeed less than 400. 
    However, another possible number that fits the restrictions is 296, which is formed by 
    interchanging the last two digits. Therefore, there does exist a number, \keyword{but it 
    is not unique}, as there are two possible numbers that fit the requirements.
\end{flushleft}
\pagebreak
\item Without trying to evaluate these numbers, show that the product of two of the numbers 
$65^{1000} - 8^{2001} + 3^{177}$, $79^{2121} - 9^{2399} + 2^{2001}$, and $24^{4493} + 5^{8192} 
+ 7^{1777}$ is non-negative.
\begin{gather*}
    n_1 = 65^{1000} - 8^{2001} + 3^{177} \\
    n_2 = 24^{4493} + 5^{8192} + 7^{1777}
\end{gather*}
\begin{gather}
    (n_1 * n_2 > 0) \leftrightarrow (n_1 > 0 \wedge n_2 > 0) \vee (n_1 < 0 \wedge n_2 < 0) \\
    n_2 > 0 = T \because (24^{4493} > 0) \wedge (5^{8192} > 0) \wedge (7^{1777} > 0) \\
    \therefore (n_1 < 0 \wedge n_2 < 0) = F, \; (n_1 > 0 \wedge n_2 > 0) \equiv (n_1 > 0) \\
    \implies (n_1 * n_2 > 0) \leftrightarrow (n_1 > 0)
\end{gather}
\begin{align}
    65^{1000} > 8^{2001} &\implies 65^{1000} + 3^{177} > 8^{2001} \\
    &\iff 65^{1000} - 8^{2001} + 3^{177} > 0
\end{align}
\begin{flushleft}
    $p$: $65^{1000} - 8^{2001} + 3^{177} > 0$ \\
    $q$: $65^{1000} + 3^{177} > 8^{2001}$ \\
    $r$: $65^{1000} > 8^{2001}$ \\
    $s$: $(n_1 * n_2 > 0)$
\end{flushleft}
\begin{gather*}
    r \then q \qquad \text{(From equation 5)} \\
    q \leftrightarrow p \qquad \text{(From equation 6)} \\
    p \leftrightarrow s \qquad \text{(From equation 4)} \\
    \therefore r \then s
\end{gather*}
\begin{align*}
    \begin{split}
        & 65^{1000} > 8^{2001} \\
        &= (64 + 1)^{1000} > 8^{2(1000.5)} \\
        &= (64 + 1)^{1000} > (8^2)^{1000.5} \\
        &= (64 + 1)^{1000} > (64)^{1000.5} \\
        &= (64 + 1)^{1000} > 64^{0.5}(64)^{1000} \\
        &= (64 + 1)^{1000} > 8(64)^{1000} \\
        &= \sqrt{65}(64 + 1)^{999.5} > 8(64)^{1000} \\
        &= \sqrt{65}(64 + 1)^{999.5} > 8(64)^{1000} \\
    \end{split}
\end{align*}
\begin{gather*}
    \sqrt{65} > \sqrt{64} = 8 \\
    \therefore (8(64 + 1)^{999.5} > 8(64)^{1000}) \then (\sqrt{65}(64 + 1)^{999.5} > 8(64)^{1000})
\end{gather*}
\begin{align*}
    \begin{split}
        & 8(64 + 1)^{999.5} > 8(64)^{1000} \\
        &\iff (64 + 1)^{999.5} > (64)^{1000} \\
        &\iff 999.5\ln(65) > 1000\ln(64) \\
        &\iff \frac{\ln(65)}{\ln(64)} > \frac{1000}{999.5} \quad [1.003727969 > 1.00050025] \qed
    \end{split}
\end{align*}
\begin{flushleft}
    Since we have found a demonstrably true statement ($\frac{\ln(65)}{\ln(64)} > \frac{1000}{999.5}$) 
    and it is logically equivalent to $8(64 + 1)^{999.5} > 8(64)^{1000}$, this statement must 
    be true, which implies that $\sqrt{65}(64 + 1)^{999.5} > 8(64)^{1000}$ is true. Since this 
    statement is ultimately equivalent to our original $r$, $r$ must be true. Finally, we showed 
    that the biconditional statement $r \leftrightarrow s$ is true, so $s$ our original 
    statement that the product of the two numbers we chose is positive is also true.
\end{flushleft}
\end{enumerate}
\end{document}